ulib/LowStar.RST.fst
@@ -27,6 +27,25 @@ open LowStar.Resource
 let r_pre (res:resource) = imem (inv res) -> Type0
 let r_post (res:resource) (a:Type) = imem (inv res) -> a -> imem (inv res) -> Type0
 
+abstract
+let rst_inv (res:resource) (h:HS.mem) =
+  B.loc_includes (B.loc_not_unused_in h) (as_loc (fp res))
+
+let reveal_rst_inv ()
+  : Lemma (forall res h . 
+             rst_inv res h 
+             <==>
+             B.loc_includes (B.loc_not_unused_in h) (as_loc (fp res)))
+  = ()
+
+(* Additional (currently assumed) lemma: 
+     Reasonable when addresses are not reused after deallocation, 
+     but currently not provided by the LowStar.Buffer library
+     (Nik and/or Tahina will look into adding it to ulib) *)
+assume val lemma_loc_not_unused_in_modifies (l:B.loc) (h0 h1:HS.mem)
+  : Lemma (requires (B.loc_includes (B.loc_not_unused_in h0) l /\ B.modifies l h0 h1))
+          (ensures  (B.loc_includes (B.loc_not_unused_in h1) l))
+
 effect RST (a:Type)
            (res:resource)
            (pre:r_pre res)
@@ -34,16 +53,18 @@ effect RST (a:Type)
        STATE a
             (fun (k:a -> HS.mem -> Type)
                (h0:HS.mem) ->
-               inv res h0 /\               //Require the resource invariant
-               pre h0 /\                   //Require the pre-condition
+               inv res h0 /\                 //Require the resource invariant
+               rst_inv res h0 /\             //Require the additional footprints invariant
+               pre h0 /\                     //Require the pre-condition
                (forall (x:a) (h1:HS.mem).
-                 inv res h1 /\                          //Ensure the resource invariant
-                 modifies res h0 h1 /\                  //Ensure that only resource's footprint is modified
-                 post h0 x h1 ==>                       //Ensure the post-condition
-                 k x h1))                               //prove the continuation under this hypothesis
+                 inv res h1 /\               //Ensure the resource invariant
+                 rst_inv res h1 /\           //Ensure the additional footprints invariant
+                 modifies res h0 h1 /\       //Ensure that only resource's footprint is modified
+                 post h0 x h1 ==>            //Ensure the post-condition
+                 k x h1))                    //prove the continuation under this hypothesis
 
 (* Left and right framing operations for RST computations *)
-
+(*
 unfold
 let frame_left_pre (#fp:resource)
                    (#frame:resource)
@@ -74,7 +95,14 @@ let frame_left (#frame:resource)
   reveal_view ();
   reveal_star ();
   reveal_modifies ();
-  f ()
+  let h0 = get () in 
+  assert (B.loc_disjoint (as_loc fp.view.fp) (as_loc frame.view.fp));
+  assert ((B.loc_unused_in h0) `B.loc_includes` (B.loc_union (as_loc fp.view.fp) (as_loc frame.view.fp)));
+  let x = f () in
+  let h1 = get () in 
+  assert ((B.loc_unused_in h1) `B.loc_includes` (as_loc (fp.view.fp)));
+  assume ((B.loc_unused_in h1) `B.loc_includes` (B.loc_union (as_loc fp.view.fp) (as_loc frame.view.fp)));
+  x
 
 unfold
 let frame_right_pre (#frame:resource)
@@ -107,6 +135,7 @@ let frame_right (#frame:resource)
   reveal_star ();
   reveal_modifies ();
   f ()
+*)
 
 (* Generic frame operation for RST computations (through resource inclusion) *)
 
@@ -129,7 +158,7 @@ let frame_post (#outer:resource)
                (h1:imem (inv outer)) = 
   post h0 x h1 /\
   sel (view_of delta) h0 == sel (view_of delta) h1
-  
+
 let frame (#a:Type)
           (#outer:resource)
           (#inner:resource)
@@ -141,7 +170,11 @@ let frame (#a:Type)
                       (frame_post delta post) =
   reveal_view ();
   reveal_modifies ();
-  f ()
+  let h0 = get () in
+  let x = f () in
+  let h1 = get () in
+  lemma_loc_not_unused_in_modifies (as_loc (fp outer)) h0 h1;
+  x
 
 (* Weaker form of framing, a bit similar to snapshot restoration in monotonic state, 
    in that the additional condition required of the inner postcondition (inner_post) 
@@ -156,10 +189,6 @@ let weak_frame_pre (#outer:resource)
                    (h:imem (inv outer)) =
   pre h
 
-// The postcondition of the inner computation has to allow us to restore the outer invariant
-let inner_post inner outer a = 
-  post:r_post inner a{forall h0 x h1 . inv outer h0 /\ post h0 x h1 ==> inv outer h1}
-
 unfold
 let weak_frame_post (#outer:resource)
                     (#inner:resource)
@@ -171,16 +200,24 @@ let weak_frame_post (#outer:resource)
                     (h1:imem (inv outer)) = 
   post h0 x h1 /\
   sel (view_of delta) h0 == sel (view_of delta) h1
-  
+
+// The postcondition of the inner computation has to allow us to restore the outer invariant
+let weak_inner_post inner outer a = 
+  post:r_post inner a{forall h0 x h1 . inv outer h0 /\ post h0 x h1 ==> inv outer h1}
+
 let weak_frame (#a:Type)
                (#outer:resource)
                (#inner:resource)
                (delta:r_weakly_includes outer inner)  // eventually we will want to infer this argument through metaprogramming
                (#pre:r_pre inner)
-               (#post:inner_post inner outer a)
+               (#post:weak_inner_post inner outer a)
                ($f:unit -> RST a inner pre post)
              : RST a outer (weak_frame_pre delta pre) 
                            (weak_frame_post delta post) =
   reveal_view ();
   reveal_modifies ();
-  f ()
+  let h0 = get () in
+  let x = f () in
+  let h1 = get () in
+  lemma_loc_not_unused_in_modifies (as_loc (fp outer)) h0 h1;
+  x
